\section{Frequenzbereich}\label{sec:ag3_2}
a)
\begin{gather*}
\alpha(t)=-kx(t)+cos(\omega t)\\
x(t)=e{^-k(t-t_0)}(x_0)+\int_{t_0}^{t} e^{k(s-t_0)}cos(\omega s)ds\\
f'=e^{k(s-t_0)}\\
g=cos(\omega s)\\
\end{gather*}
partiell integrieren
\begin{gather*}
f=\frac{e^{k(s-t_0)}}{k}\\
g'=-\omega sind(\omega s)\\
(e^{-k(t-t_0)}x_0)+[\frac{e^{k(t-t_0)}cos(\omega s)}{k}]^{s=t}_{s=t_0}-\int_{t_0}^{t}-\frac{\omega sin(\omega s)e^{k(s-t_0)}}{k}ds\\
\end{gather*}
partiell integrieren
\begin{gather*}
f'=\frac{e^{k(s-t_0)}}{k}\\
g=-\omega sin(\omega s)\\
f=\frac{e^{k(s-t_0)}}{k^2}\\
g'=-\omega^2 sin(\omega s)\\
\end{gather*}
\begin{gather*}
(e^{-k(t-t_0)}x_0)+[\frac{e^{k(t-t_0)}cos(\omega s)}{k}]^{t}_{s=t_0}-(-[\frac{\omega^{k(s-t_0)}sin(\omega s)}{k^2}]^{t}_{s=t_0}\int_{t_0}^{t}-\frac{\omega^2 e^{k(s-t_0)}cos(\omega s)}{k^2}ds)\\
(e^{-k(t-t_0)}x_0)+\int_{t_0}^{t}e^{k(s-t_0)}cos(\omega s)ds=[\frac{e^{k(t-t_0)}cos(\omega s)}{k}]^{t}_{s=t_0}+[\frac{\omega^{k(s-t_0)}sin(\omega s)}{k^2}]^{t}_{s=t_0}-\frac{\omega^2}{h^2}\int_{t}^{s=t_0}e^{k(s-t_0)}cos(\omega s)ds\\
\int_{t_0}^{t}e^{k(s-t_0)}cos(\omega s)ds+\frac{\omega^2}{k^2}\int_{t}^{t_0}e^{k(s-t_0)}cos(\omega s)ds=[\frac{e^{k(s-t_0)}cos(\omega s)}{k}]^{t}_{s=t_0}+[\frac{\omega e^{k(s-t_0)}sin(\omega s)}{k^2}]^{t}_{s=t_0}\\
\int_{t_0}^{t}e^{k(s-t_0)}cos(\omega s)ds+(1+\frac{\omega^2}{h^2})=[\frac{e^{k(t-t_0)}cos(\omega s)}{k}]^{t}_{s=t_0}+[\frac{\omega e^{k(s-t_0)}sin(\omega s)}{k^2}]^{t}_{s=t_0}\\
\int_{t_0}^{t}e^{k(s-t_0)}cos(\omega s)ds+(\frac{k^2+\omega^2}{h^2})=[\frac{e^{k(t-t_0)}cos(\omega s)}{k}]^{t}_{s=t_0}+[\frac{\omega e^{k(s-t_0)}sin(\omega s)}{k^2}]^{t}_{s=t_0}\\
\int_{t_0}^{t}e^{k(s-t_0)}cos(\omega s)ds=([\frac{e^{k(t-t_0)}cos(\omega s)}{k}]^{t}_{s=t_0}+[\frac{\omega e^{k(s-t_0)}sin(\omega s)}{k^2}]^{t}_{s=t_0})*(\frac{k^2+\omega^2}{h^2})\\
=[\frac{ke^{k(t-t_0)}cos(\omega s)+\omega e^{k(s-t_0)}sin(\omega s)}{\omega^2+k^2}]^{t}_{s=t_0}\\
=\frac{[e^{k(t-t_0)}cos(\omega s)+\omega e^{k(s-t_0)}sin(\omega s)]^{t}_{s=t_0}}{\omega^2+k^2}\\
e^{-kt+kt_0}=\frac{e^{kt_0}}{e^{kt}}\\
=\frac{\omega e^{kt}sin(\omega t)+ke^{kt}cos(\omega t)}{e^{kt_0}(\omega^2+k^2)}-\frac{\omega sin(\omega t_0)+kcos(\omega t_0)}{(\omega^2+k^2)}\\
x(t)=e^{-k(t-t_0)}(x_0+\frac{\omega e^{kt}sin(\omega t)+ke^{kt}cos(\omega t)}{e^{kt_0}(\omega^2+k^2)}-\frac{\omega sin(\omega t_0)+kcos(\omega t_0)}{(\omega^2+k^2)})\\
=\frac{\omega sin(\omega t)+kcos(\omega t)}{(\omega^2+k^2)}-e^{-k(t-t_0)}(\frac{\omega sin(\omega t_0)+kcos(\omega t_0)}{(\omega^2+k^2)}-x_0)\\
=e^{-k(t-7_0)}(x_0-\frac{\omega sin(\omega t_0)+kcos(\omega t_0)}{(\omega^2+k^2)})+\frac{\omega sin(\omega t)+kcos(\omega t)}{(\omega^2+k^2)}
\end{gather*}